tidy and shuffle

isabelle/CVM_Original/Utils/PMF/Utils_PMF_Basic.thy
@@ -16,28 +16,11 @@ lemma pmf_map_pred_true_eq_prob :
   \<open>pmf (map_pmf P p) True = \<P>(x in measure_pmf p. P x)\<close>
   by (simp add: measure_pmf_cong pmf_map)
 
-(* abbreviation (input) kleisli_compose_left ::
-  \<open>('a \<Rightarrow> 'b pmf) \<Rightarrow> ('b \<Rightarrow> 'c pmf) \<Rightarrow> 'a \<Rightarrow> 'c pmf\<close>
-  (infixl \<open>>=>\<close> 50) where
-  \<open>(f >=> g) \<equiv> \<lambda> x. bind_pmf (f x) g\<close>
-
-abbreviation (input) kleisli_compose_right ::
-  \<open>('b \<Rightarrow> 'c pmf) \<Rightarrow> ('a \<Rightarrow> 'b pmf) \<Rightarrow> 'a \<Rightarrow> 'c pmf\<close>
-  (infixr \<open><=<\<close> 50) where
-  \<open>(f <=< g) \<equiv> g >=> f\<close> *)
-
-abbreviation \<open>foldM_pmf \<equiv> foldM bind_pmf return_pmf\<close>
-abbreviation \<open>foldM_pmf_enumerate \<equiv> foldM_enumerate bind_pmf return_pmf\<close>
-
 lemma map_pmf_times_one [simp] :
   fixes p :: \<open>nat pmf\<close>
   shows \<open>map_pmf ((*) <| Suc 0) p = p\<close>
   by (simp add: pmf.map_ident_strong)
 
-lemma foldM_pmf_snoc :
-  "foldM_pmf f (xs@[y]) val = bind_pmf (foldM_pmf f xs val) (f y)"
-  by (induction xs arbitrary:val)
-    (simp_all add: bind_return_pmf bind_return_pmf' bind_assoc_pmf cong:bind_pmf_cong)
 
 lemma prod_pmf_reindex :
   assumes "finite T" "f ` S \<subseteq> T" "inj_on f S"
@@ -86,6 +69,8 @@ lemma bool_pmf_eqI :
   assumes "pmf p True = pmf q True"
   shows "p = q"
   using assms pmf_False_conv_True by (intro pmf_eqI) (metis (full_types))
+
+section \<open>Properties about Pi_pmf and prod_pmf\<close>
 
 text \<open>Better version of Pi_pmf_map.\<close>
 lemma Pi_pmf_map' :
@@ -183,5 +168,151 @@ proof -
   
   finally show ?thesis .
 qed
+
+section \<open>Properties about the Bernoulli and Binomial distributions\<close>
+
+lemma bernoulli_pmf_0_1 [simp] :
+  \<open>bernoulli_pmf 0 = return_pmf False\<close>
+  \<open>bernoulli_pmf 1 = return_pmf True\<close>
+  by (simp_all add: bernoulli_pmf.rep_eq pmf_eqI)
+
+lemma
+  binomial_pmf_p_0 [simp] : \<open>binomial_pmf n 0 = return_pmf 0\<close> and
+  binomial_pmf_p_1 [simp] : \<open>binomial_pmf n 1 = return_pmf n\<close>
+  using set_pmf_subset_singleton by fastforce+
+
+context
+  fixes p :: real
+  assumes p [simp] : \<open>0 \<le> p\<close> \<open>p \<le> 1\<close>
+begin
+
+lemma bernoulli_pmf_eq_bernoulli_pmfs :
+  assumes \<open>0 \<le> p'\<close> \<open>p' \<le> 1\<close>
+  shows
+    \<open>bernoulli_pmf (p * p') = do {
+      b \<leftarrow> bernoulli_pmf p;
+      b' \<leftarrow> bernoulli_pmf p';
+      return_pmf <| b \<and> b' }\<close>
+  using assms p
+  apply (intro pmf_eqI)
+  by (simp add: mult_le_one bernoulli_pmf.rep_eq pmf_bind algebra_simps)
+
+lemmas bernoulli_pmf_eq_bernoulli_pmfs' = bernoulli_pmf_eq_bernoulli_pmfs[
+  simplified map_pmf_def[symmetric]]
+
+private lemma bernoulli_eq_map_Pi_pmf_aux : 
+  assumes \<open>card I = Suc k\<close>
+  shows
+    \<open>bernoulli_pmf (p ^ Suc k) = (
+      \<lblot>bernoulli_pmf p\<rblot>
+        |> Pi_pmf I dflt
+        |> map_pmf (Ball I))\<close>
+    (is \<open>?L k = ?R I\<close>)
+using assms proof (induction k arbitrary: I)
+  case 0
+  then show ?case
+    by (auto simp add: Pi_pmf_singleton card_1_singleton_iff map_pmf_comp)
+next
+  case (Suc k)
+  moreover from calculation obtain x J where
+    \<open>finite J\<close> \<open>card J = Suc k\<close> \<open>I = insert x J\<close> \<open>x \<notin> J\<close>
+    by (metis card_Suc_eq_finite)
+
+  moreover from calculation have
+    \<open>?L (Suc k)  = do {
+      b \<leftarrow> bernoulli_pmf p;
+      b' \<leftarrow> ?R J;
+      return_pmf <| b \<and> b' }\<close>
+    by (simp add: bernoulli_pmf_eq_bernoulli_pmfs mult_le_one power_le_one_iff)
+
+  moreover from calculation
+  have \<open>\<dots> = ?R (insert x J)\<close>
+    apply (subst Pi_pmf_insert')
+    by (auto
+      intro: bind_pmf_cong map_pmf_cong
+      simp flip: map_pmf_def
+      simp add: map_pmf_comp map_bind_pmf)
+
+  ultimately show ?case by simp
+qed
+
+text
+  \<open>This says that to simulate a coin flip with the probability of getting H as
+  p ^ k, we can flip \<ge> k coins with probability p of getting H, and check if
+  any k of them are H. 
+
+  More precisely, a bernoulli RV with probability p ^ k (k > 0) is equivalent
+  to doing the following:
+  1. We fix a (finite) family of indices J, and a subset I \<subseteq> J of cardinality k.
+  2. We construct a family of IID bernoulli RVs of probability p,
+     indexed by J, and sample from it.
+  3. Viewing the outcome as a characteristic function of J, we check if the
+     subset it defines contains I, outputting \<top> iff that is the case.\<close>
+lemma bernoulli_eq_map_Pi_pmf :
+  assumes \<open>finite J\<close> \<open>card I > 0\<close> \<open>I \<subseteq> J\<close>
+  shows
+    \<open>bernoulli_pmf (p ^ card I) = (
+      \<lblot>bernoulli_pmf p\<rblot>
+        |> Pi_pmf J dflt
+        |> map_pmf (Ball I))\<close>
+  using
+    assms p 
+    bernoulli_eq_map_Pi_pmf_aux[of I \<open>card I - 1\<close> dflt]
+    Pi_pmf_subset[of J I dflt \<open>\<lblot>bernoulli_pmf p\<rblot>\<close>]
+  by (fastforce simp add: map_pmf_comp)
+
+end
+
+abbreviation bernoulli_nat_pmf :: \<open>real \<Rightarrow> nat pmf\<close> where
+ \<open>bernoulli_nat_pmf \<equiv> bernoulli_pmf >>> map_pmf of_bool\<close>
+
+context binomial_distribution
+begin
+
+abbreviation Pi_bernoulli_nat_pmf :: \<open>(nat \<Rightarrow> nat) pmf\<close> where
+  \<open>Pi_bernoulli_nat_pmf \<equiv> Pi_pmf {..< n} 0 \<lblot>bernoulli_nat_pmf p\<rblot>\<close>
+
+lemma binomial_pmf_eq_map_sum_of_bernoullis :
+  \<open>binomial_pmf n p = (
+    Pi_bernoulli_nat_pmf
+      |> map_pmf (\<lambda> P. \<Sum> m < n. P m))\<close>
+  (is \<open>?L = ?R\<close>)
+proof -
+  from p have \<open>?L = (
+    prod_pmf {..< n} \<lblot>bernoulli_pmf p\<rblot>
+      |> map_pmf (\<lambda> P. card {m. m < n \<and> P m}))\<close>
+    apply (subst binomial_pmf_altdef'[where A = \<open>{..< n}\<close> and dflt = undefined])
+    by simp_all
+
+  also have \<open>\<dots> = ?R\<close>
+    unfolding Pi_pmf_map'[OF finite_lessThan, where dflt' = undefined] map_pmf_comp
+    by (fastforce simp add: Collect_conj_eq lessThan_def)
+
+  finally show ?thesis .
+qed
+
+lemma expectation_binomial_pmf :
+  \<open>measure_pmf.expectation (binomial_pmf n p) id = n * p\<close>
+  using p
+  by (simp add:
+    binomial_pmf_eq_map_sum_of_bernoullis
+    expectation_sum_Pi_pmf integrable_measure_pmf_finite)
+
+end
+
+definition bernoulli_matrix ::
+  \<open>nat \<Rightarrow> nat \<Rightarrow> real \<Rightarrow> (nat \<times> nat \<Rightarrow> bool) pmf\<close> where
+  \<open>bernoulli_matrix m n p \<equiv>
+    prod_pmf ({..< m} \<times> {..< n}) \<lblot>bernoulli_pmf p\<rblot>\<close>
+
+lemma bernoulli_matrix_eq_uncurry_prod :
+  fixes m n
+  defines \<open>m' \<equiv> {..< m}\<close> and \<open>n' \<equiv> {..< n}\<close>
+  shows
+    \<open>bernoulli_matrix m n p = (
+      prod_pmf m' \<lblot>prod_pmf n' \<lblot>bernoulli_pmf p\<rblot>\<rblot>
+        |> map_pmf (\<lambda> \<omega>. \<lambda> (x, y) \<in> m' \<times> n'. \<omega> x y))\<close>
+  unfolding bernoulli_matrix_def m'_def n'_def
+  by (simp add: prod_pmf_uncurry)
 
 end
